feat(library/type_context): unfold lemmas in major premise of acc.rec

src/library/constants.cpp
@@ -6,6 +6,7 @@ namespace lean{
 name const * g_abs = nullptr;
 name const * g_absurd = nullptr;
 name const * g_acc_cases_on = nullptr;
+name const * g_acc_rec = nullptr;
 name const * g_add_comm_group = nullptr;
 name const * g_add_comm_semigroup = nullptr;
 name const * g_add_group = nullptr;
@@ -379,6 +380,7 @@ void initialize_constants() {
     g_abs = new name{"abs"};
     g_absurd = new name{"absurd"};
     g_acc_cases_on = new name{"acc", "cases_on"};
+    g_acc_rec = new name{"acc", "rec"};
     g_add_comm_group = new name{"add_comm_group"};
     g_add_comm_semigroup = new name{"add_comm_semigroup"};
     g_add_group = new name{"add_group"};
@@ -753,6 +755,7 @@ void finalize_constants() {
     delete g_abs;
     delete g_absurd;
     delete g_acc_cases_on;
+    delete g_acc_rec;
     delete g_add_comm_group;
     delete g_add_comm_semigroup;
     delete g_add_group;
@@ -1126,6 +1129,7 @@ void finalize_constants() {
 name const & get_abs_name() { return *g_abs; }
 name const & get_absurd_name() { return *g_absurd; }
 name const & get_acc_cases_on_name() { return *g_acc_cases_on; }
+name const & get_acc_rec_name() { return *g_acc_rec; }
 name const & get_add_comm_group_name() { return *g_add_comm_group; }
 name const & get_add_comm_semigroup_name() { return *g_add_comm_semigroup; }
 name const & get_add_group_name() { return *g_add_group; }
