src/library/type_context.cpp
@@ -756,6 +756,18 @@ optional<expr> type_context::reduce_aux_recursor(expr const & e) {
         return none_expr();
 }
 
+optional<expr> type_context::reduce_large_elim_recursor(expr const & e) {
+    expr const & f = get_app_fn(e);
+    if (!is_constant(f))
+        return none_expr();
+    auto & fn = const_name(f);
+    if (fn == get_acc_rec_name()) {
+        transparency_scope scope(*this, transparency_mode::All);
+        return norm_ext(e);
+    }
+    return none_expr();
+}
+
 bool type_context::should_unfold_macro(expr const & e) {
     /* If m_transparency_mode is set to ALL, then we unfold all
        macros. In this way, we make sure type inference does not fail.
@@ -881,9 +893,14 @@ expr type_context::whnf_core(expr const & e0, bool proj_reduce) {
             if (auto r = reduce_aux_recursor(e)) {
                 e = *r;
                 continue;
-            } else {
-                return e;
             }
+
+            if (auto r = reduce_large_elim_recursor(e)) {
+                e = *r;
+                continue;
+            }
+
+            return e;
         } else {
             e = mk_rev_app(f, args.size(), args.data());
             continue;
