tests/lean/run/unfold_lemmas.lean
@@ -1,10 +1,10 @@
 open nat well_founded
 
-def gcd.F : Π (y : ℕ), (Π (y' : ℕ), y' < y → nat → nat) → nat → nat
-| 0        f x := x
-| (succ y) f x := f (x % succ y) (mod_lt _ $ succ_pos _) (succ y)
+def gcd : ℕ → ℕ → ℕ | y := λ x,
+if h : y = 0 then
+    x
+else
+    have x % y < y, by { apply mod_lt, cases y, contradiction, apply succ_pos },
+    gcd (x % y) y
 
-def gcd (x y : nat) := fix lt_wf gcd.F y x
-
-set_option type_context.unfold_lemmas true
-@[simp] lemma gcd_zero_right (x : nat) : gcd x 0 = x := rfl
+@[simp] lemma gcd_zero_right (x : nat) : gcd 0 x = x := rfl
