tests/lean/run/check_constants.lean
@@ -6,6 +6,7 @@ do env ← get_env, (env^.get n >> return ()) <|> (guard $ env^.is_namespace n) 
 run_cmd script_check_id `abs
 run_cmd script_check_id `absurd
 run_cmd script_check_id `acc.cases_on
+run_cmd script_check_id `acc.rec
 run_cmd script_check_id `add_comm_group
 run_cmd script_check_id `add_comm_semigroup
 run_cmd script_check_id `add_group
